added simple example

examples/bls.ec
@@ -1,26 +1,75 @@
-prover alt-ergo, cvc3.
+(* prover alt-ergo, cvc3. *)
 
-type group.
+type G_1.
+type G_T.
 type message.
 type key_pair.
 type sk.
 type pk.
 
-cnst g : group.
+cnst g_1_i : G_1.
+cnst g_T_i : G_T.
+cnst g : G_1.
 cnst n : int.
 cnst dummy : message.
 cnst q : int.
 
-op [^] : (group, int) -> group as group_pow.
-op [*] : (group, group) -> group as group_mul.
-op e : (group, group) -> group as group_pair.
-op groupOp : (group, group) -> group.
+op [*] : (G_1, G_1) -> G_1 as G_1_mul.
+op [^] : (G_1, int) -> G_1 as G_1_pow.
 
-axiom group_exp_0 : forall (x : group), x ^ 1 = x.
-axiom group_exp_S : forall (x : group, k : int), k > 1 => x ^ k = groupOp(x, x^(k-1)).
+op [*] : (G_T, G_T) -> G_T as G_T_mul.
+op [^] : (G_T, int) -> G_T as G_T_pow.
 
-axiom bilinear_map_0 : forall (x : group, a : int), e(x ^ a, x) = e(x, x) ^ a.
-axiom bilinear_map_1 : forall (x : group, b : int), e(x, x ^ b) = e(x, x) ^ b.
-axiom bilinear_map_2 : forall (x : group, y : group, a : int, b : int), e(x ^ a, y ^ b) = e(x, y) ^ (a * b).
+op e : (G_1, G_1) -> G_T as G_1_pair.
+
+axiom G_1_mult_1 : forall (x : G_1), x * g_1_i = x.
+axiom G_1_exp_0 : forall (x : G_1), x ^ 0 = g_1_i.
+axiom G_1_exp_S : forall (x : G_1, k : int), k > 0 => x ^ k = x * (x^(k-1)).
+
+axiom G_T_mult_1 : forall (x : G_T), x * g_T_i = x.
+axiom G_T_exp_0 : forall (x : G_T), x ^ 0 = g_T_i.
+axiom G_T_exp_S : forall (x : G_T, k : int), k > 0 => x ^ k = x * (x^(k-1)).
 
 
+axiom bilinearity : forall (x : G_1, y : G_1, a : int, b : int), e(x ^ a, y ^ b) = e(x, y) ^ (a * b).
+
+adversary A (g : G_1, x : G_T) : bool {}.
+
+cnst a : int.
+cnst b : int.
+
+game G3 = {
+
+  abs A = A{}
+
+  fun Main() : G_T = {
+    var ret : G_T;
+    ret = e(g^a, g^b);
+    return ret;
+  }
+
+  fun Experiment() : bool = {
+    var x : G_T;
+    var decision : bool;
+
+    x = Main();
+    decision = A(g, x);
+    return (decision = true);
+  }
+}.
+
+game G4 = G3 
+where Main = {
+    var ret : G_T;
+    ret = (e(g, g))^(b * a);
+    return ret;
+}.
+ 
+
+equiv g3_g4_equiv: G3.Main ~ G4.Main : true ==> ={res}.
+trivial.
+save.
+
+equiv g3_g4_equiv_exp: G3.Experiment ~ G4.Experiment : true ==> ={res}.
+call.
+call using g3_g4_equiv.
