examples/simple.ec
@@ -1,0 +1,76 @@
+(* prover alt-ergo, cvc3. *)
+
+type group.
+
+adversary A() : int {}.
+
+game simple = {
+
+  abs A  = A {}
+
+  fun Main() : bool = {
+    var x : int;
+    var y : int;
+
+
+    y=4;
+    x = A();
+    return (x=5);
+  }
+
+  fun new() : bool = {
+    return true;
+  }
+}.
+
+
+game simple2 = simple
+
+
+  where Main = {
+  var x : int;
+  var y : int;
+
+  y=5;
+  x=A();
+  return (x=5);
+}.
+
+
+(* equiv A_and_A : simple.A ~ simple2.A: true ==> ={res}. *)
+
+
+equiv simple1_2 : simple.Main ~ simple2.Main: true ==> ={res}.
+call.
+trivial.
+save.
+
+game testcall = simple
+where new = {
+  var b: bool;
+
+  b=Main();
+  return b;
+}.
+
+game testcall2 = simple2
+where new = {
+  var b: bool;
+  var z: int;
+
+  z=6;
+
+  b=Main();
+  return b;
+}. 
+
+equiv tmain1_2 : testcall.Main ~ testcall2.Main: true ==> ={res}.
+call.
+trivial. 
+save.
+
+
+equiv new1_2 : testcall.new ~ testcall2.new: true ==> ={res}.
+call using tmain1_2.
+trivial.
+
